final removal of local tries

thys/Collections/Lib/Assoc_List.thy
@@ -5,86 +5,6 @@ theory Assoc_List
   "../Iterator/SetIteratorOperations"
 begin
 
-subsection {* Additional operations for associative lists *}
-
-primrec update_with_aux :: "'val \<Rightarrow> 'key \<Rightarrow> ('val \<Rightarrow> 'val) \<Rightarrow> ('key \<times> 'val) list \<Rightarrow> ('key \<times> 'val) list"
-where
-  "update_with_aux v k f [] = [(k, f v)]"
-| "update_with_aux v k f (p # ps) = (if (fst p = k) then (k, f (snd p)) # ps else p # update_with_aux v k f ps)"
-
-text {*
-  Do not use @{term "AList.delete"} because this traverses all the list even if it has found the key.
-  We do not have to keep going because we use the invariant that keys are distinct.
-*}
-fun delete_aux :: "'key \<Rightarrow> ('key \<times> 'val) list \<Rightarrow> ('key \<times> 'val) list"
-where
-  "delete_aux k [] = []"
-| "delete_aux k ((k', v) # xs) = (if k = k' then xs else (k', v) # delete_aux k xs)"
-
-lemma map_of_update_with_aux':
-  "map_of (update_with_aux v k f ps) k' = ((map_of ps)(k \<mapsto> (case map_of ps k of None \<Rightarrow> f v | Some v \<Rightarrow> f v))) k'"
-by(induct ps) auto
-
-lemma map_of_update_with_aux:
-  "map_of (update_with_aux v k f ps) = (map_of ps)(k \<mapsto> (case map_of ps k of None \<Rightarrow> f v | Some v \<Rightarrow> f v))"
-by(simp add: fun_eq_iff map_of_update_with_aux')
-
-lemma dom_update_with_aux: "fst ` set (update_with_aux v k f ps) = {k} \<union> fst ` set ps"
-  by (induct ps) auto
-
-lemma distinct_update_with_aux [simp]:
-  "distinct (map fst (update_with_aux v k f ps)) = distinct (map fst ps)"
-by(induct ps)(auto simp add: dom_update_with_aux)
-
-lemma set_update_with_aux:
-  "distinct (map fst xs) 
-  \<Longrightarrow> set (update_with_aux v k f xs) = (set xs - {k} \<times> UNIV \<union> {(k, f (case map_of xs k of None \<Rightarrow> v | Some v \<Rightarrow> v))})"
-by(induct xs)(auto intro: rev_image_eqI)
-
-lemma set_delete_aux: "distinct (map fst xs) \<Longrightarrow> set (delete_aux k xs) = set xs - {k} \<times> UNIV"
-apply(induct xs)
-apply simp_all
-apply clarsimp
-apply(fastforce intro: rev_image_eqI)
-done
-
-lemma dom_delete_aux: "distinct (map fst ps) \<Longrightarrow> fst ` set (delete_aux k ps) = fst ` set ps - {k}"
-by(auto simp add: set_delete_aux)
-
-lemma distinct_delete_aux [simp]:
-  "distinct (map fst ps) \<Longrightarrow> distinct (map fst (delete_aux k ps))"
-proof(induct ps)
-  case Nil thus ?case by simp
-next
-  case (Cons a ps)
-  obtain k' v where a: "a = (k', v)" by(cases a)
-  show ?case
-  proof(cases "k' = k")
-    case True with Cons a show ?thesis by simp
-  next
-    case False
-    with Cons a have "k' \<notin> fst ` set ps" "distinct (map fst ps)" by simp_all
-    with False a have "k' \<notin> fst ` set (delete_aux k ps)"
-      by(auto dest!: dom_delete_aux[where k=k])
-    with Cons a show ?thesis by simp
-  qed
-qed
-
-lemma map_of_delete_aux':
-  "distinct (map fst xs) \<Longrightarrow> map_of (delete_aux k xs) = (map_of xs)(k := None)"
-  apply (induct xs)
-  apply (fastforce intro: ext simp add: map_of_eq_None_iff fun_upd_twist)
-  apply (auto intro!: ext simp del: map_upd_eq_restrict )
-  apply (simp add: map_of_eq_None_iff)
-  done
-
-lemma map_of_delete_aux:
-  "distinct (map fst xs) \<Longrightarrow> map_of (delete_aux k xs) k' = ((map_of xs)(k := None)) k'"
-by(simp add: map_of_delete_aux')
-
-lemma delete_aux_eq_Nil_conv: "delete_aux k ts = [] \<longleftrightarrow> ts = [] \<or> (\<exists>v. ts = [(k, v)])"
-by(cases ts)(auto split: split_if_asm)
-
 subsection {* Type @{text "('a, 'b) assoc_list" } *}
 
 typedef ('k, 'v) assoc_list = "{xs :: ('k \<times> 'v) list. distinct (map fst xs)}"
@@ -116,10 +36,10 @@ definition lookup :: "('k, 'v) assoc_list \<Rightarrow> 'k \<Rightarrow> 'v opti
 where [code]: "lookup al = map_of (impl_of al)" 
 
 definition update_with :: "'v \<Rightarrow> 'k \<Rightarrow> ('v \<Rightarrow> 'v) \<Rightarrow> ('k, 'v) assoc_list \<Rightarrow> ('k, 'v) assoc_list"
-where [code del]: "update_with v k f al = Assoc_List (update_with_aux v k f (impl_of al))"
+where [code del]: "update_with v k f al = Assoc_List (AList.update_with_aux v k f (impl_of al))"
 
 definition delete :: "'k \<Rightarrow> ('k, 'v) assoc_list \<Rightarrow> ('k, 'v) assoc_list"
-where [code del]: "delete k al = Assoc_List (delete_aux k (impl_of al))"
+where [code del]: "delete k al = Assoc_List (AList.delete_aux k (impl_of al))"
 
 definition iteratei :: "('k, 'v) assoc_list \<Rightarrow> ('s\<Rightarrow>bool) \<Rightarrow> ('k \<times> 'v \<Rightarrow> 's \<Rightarrow> 's) \<Rightarrow> 's \<Rightarrow> 's" 
 where [code]: "iteratei al c f = foldli (impl_of al) c f"
@@ -128,11 +48,11 @@ lemma impl_of_empty [code abstract]: "impl_of empty = []"
 by(simp add: empty_def Assoc_List_inverse)
 
 lemma impl_of_update_with [code abstract]:
-  "impl_of (update_with v k f al) = update_with_aux v k f (impl_of al)"
+  "impl_of (update_with v k f al) = AList.update_with_aux v k f (impl_of al)"
 by(simp add: update_with_def Assoc_List_inverse)
 
 lemma impl_of_delete [code abstract]:
-  "impl_of (delete k al) = delete_aux k (impl_of al)"
+  "impl_of (delete k al) = AList.delete_aux k (impl_of al)"
 by(simp add: delete_def Assoc_List_inverse)
 
 subsection {* Abstract operation properties *}
